Minor changes

src/set.dfy
@@ -20,3 +20,51 @@ function Union<T>(s1: set<T>, s2: set<T>): set<T>
 {
   set x | x in s1 || x in s2
 }
+
+
+// references: 
+// https://stackoverflow.com/questions/50195891/how-do-i-write-a-clean-function-in-dafny-to-get-the-minimum-of-a-set
+// https://stackoverflow.com/questions/49398650/dafny-what-does-no-terms-found-to-trigger-on-mean
+
+// A trigger is a syntactic pattern involving quantified variables that serves as heuristic for the solver to do something with the quantifier. 
+// With a forall quantifier, the trigger tells Dafny when to instantiate the quantified formula with other expressions. 
+// Otherwise, Dafny will never use the quantified formula.
+method max(s: set<int>) returns (m: int) 
+    requires |s| > 0
+    ensures forall k :: k in s ==> k <= m
+{ 
+  var e :| e in s; // && forall k :: k in s ==> e >= k;
+  if (|s| >  1)  {
+      var r := max(s - {e});
+      m := (if e > r then  e else r);
+      
+      // postcondition is not met without this
+      // however it gives a warning: 'no terms found to trigger on'
+      assert forall k :: k in (s - {e}) ==> m >= k; 
+
+      assert m >= e;
+  } else {
+      assert |s - {e}| == 0;
+      return e;
+  }
+}
+
+function Pick(s: set<int>): int
+  requires |s| > 0
+{
+  var x :| x in s; x
+} 
+
+// taken from: http://leino.science/papers/krml274.html
+lemma Choices(s: set<int>)
+  requires s != {}
+{
+  var a := Pick(s);
+  var b := Pick(s);
+  // this is provable since the same :| operator is used
+  // Placing it in a function guarantees that on the same argument, the same results is returned on every execution
+  assert a == b;
+  a := var x :| x in s; x;
+  b := var x :| x in s; x;
+  assert a == b;  // error: not provable
+}
